Rename identifiers and make more use of field notations

Dpda/Conversion/CPSPToHopcroft.lean
@@ -6,11 +6,11 @@ import Dpda.RepeatBindMap
  - CPSP --> Hopcroft
  -/
 
-def Hopcroft_DPDA_IDesc.fromCPSP {Q S Γ} [Fintype Q] [DecidableEq Q] [Fintype S] [Fintype Γ] [DecidableEq Γ]
+def CPSP_DPDA_IDesc.toHopcroft {Q S Γ} [Fintype Q] [DecidableEq Q] [Fintype S] [Fintype Γ] [DecidableEq Γ]
   (pwβ: CPSP_DPDA_IDesc Q S Γ) : Hopcroft_DPDA_IDesc Q S (AugmentZ0 Γ) :=
   ⟨pwβ.p, pwβ.w, pwβ.β.map AugmentZ0.fromΓ ++ [AugmentZ0.z0]⟩
 
-def Hopcroft_DPDA.fromCPSP {Q S Γ} (M_tilde: CPSP_DPDA Q S Γ): Hopcroft_DPDA Q S (AugmentZ0 Γ) :=
+def CPSP_DPDA.toHopcroft {Q S Γ} (M_tilde: CPSP_DPDA Q S Γ): Hopcroft_DPDA Q S (AugmentZ0 Γ) :=
   let q0 := M_tilde.q0
   let z_0 := AugmentZ0.z0
   let F := M_tilde.F
@@ -47,24 +47,21 @@ def Hopcroft_DPDA.fromCPSP {Q S Γ} (M_tilde: CPSP_DPDA Q S Γ): Hopcroft_DPDA Q
 theorem CPSP_to_Hopcroft_preserves_semantics_single_step {Q S Γ}
   [Fintype Q] [DecidableEq Q] [Fintype S] [Fintype Γ] [DecidableEq Γ]
   (M: CPSP_DPDA Q S Γ) (idesc: CPSP_DPDA_IDesc Q S Γ) :
-  let M_hop := Hopcroft_DPDA.fromCPSP M
-  let idesc_hop := Hopcroft_DPDA_IDesc.fromCPSP idesc
-  let after_step : Option (CPSP_DPDA_IDesc Q S Γ) := CPSP_Judge.stepTransition M.transition idesc
-  let after_step_hop : Option (Hopcroft_DPDA_IDesc Q S (AugmentZ0 Γ)) := Hopcroft_DPDA.stepTransition M_hop idesc_hop
-  after_step.map Hopcroft_DPDA_IDesc.fromCPSP = after_step_hop := by
+  CPSP_DPDA_IDesc.toHopcroft <$> M.transition.stepTransition idesc = M.toHopcroft.stepTransition idesc.toHopcroft := by
+    simp only [Functor.map]
     cases h : idesc.β with
      | cons X β =>
       simp only [
-        CPSP_Judge.stepTransition,
+        CPSP_Transition.stepTransition,
         h,
         Hopcroft_DPDA.stepTransition,
-        Hopcroft_DPDA_IDesc.fromCPSP,
-        Hopcroft_DPDA.fromCPSP,
+        CPSP_DPDA_IDesc.toHopcroft,
+        CPSP_DPDA.toHopcroft,
         List.map_cons, List.cons_append]
       match M.transition (idesc.p, AugmentZ0.fromΓ X) with
       | CPSP_Judge.immediate (some (α, p)) =>
         simp only [Option.map_some, Option.some.injEq]
-        simp only [Hopcroft_DPDA_IDesc.fromCPSP, List.map_append, List.append_assoc]
+        simp only [CPSP_DPDA_IDesc.toHopcroft, List.map_append, List.append_assoc]
       | CPSP_Judge.immediate none =>
         simp only [Option.map_none]
         cases h2 : idesc.w with
@@ -82,18 +79,18 @@ theorem CPSP_to_Hopcroft_preserves_semantics_single_step {Q S Γ}
           | some u =>
             let ⟨k,l⟩ := u
             simp only [Option.map_some, Option.some.injEq]
-            simp only [Hopcroft_DPDA_IDesc.fromCPSP, List.map_append, List.append_assoc]
+            simp only [CPSP_DPDA_IDesc.toHopcroft, List.map_append, List.append_assoc]
      | nil =>
       simp only [
-        CPSP_Judge.stepTransition, h,
+        CPSP_Transition.stepTransition, h,
         Hopcroft_DPDA.stepTransition,
-        Hopcroft_DPDA_IDesc.fromCPSP,
-        Hopcroft_DPDA.fromCPSP,
+        CPSP_DPDA_IDesc.toHopcroft,
+        CPSP_DPDA.toHopcroft,
         List.map_nil, List.nil_append, List.append_nil]
       match M.transition (idesc.p, AugmentZ0.z0) with
       | CPSP_Judge.immediate (some (α, p)) =>
         simp only [Option.map_some, Option.some.injEq]
-        simp only [Hopcroft_DPDA_IDesc.fromCPSP]
+        simp only [CPSP_DPDA_IDesc.toHopcroft]
       | CPSP_Judge.immediate none =>
         simp only [Option.map_none]
         cases h2 : idesc.w with
@@ -111,32 +108,32 @@ theorem CPSP_to_Hopcroft_preserves_semantics_single_step {Q S Γ}
           | some u =>
             let ⟨k,l⟩ := u
             simp only [Option.map_some, Option.some.injEq]
-            simp only [Hopcroft_DPDA_IDesc.fromCPSP]
+            simp only [CPSP_DPDA_IDesc.toHopcroft]
 
 theorem CPSP_to_Hopcroft_preserves_semantics {Q S Γ} [Fintype Q] [DecidableEq Q] [Fintype S] [Fintype Γ] [DecidableEq Γ]
   (M: CPSP_DPDA Q S Γ) (w: List S) (n: ℕ) :
-  Hopcroft_DPDA.membership_provable_in_n_steps (Hopcroft_DPDA.fromCPSP M) w n =
+  Hopcroft_DPDA.membership_provable_in_n_steps (CPSP_DPDA.toHopcroft M) w n =
   CPSP_DPDA.membership_provable_in_n_steps M w n := by
     let α := CPSP_DPDA_IDesc Q S Γ
     let β := Hopcroft_DPDA_IDesc Q S (AugmentZ0 Γ)
-    let th : ∀ idesc, (CPSP_Judge.stepTransition M.transition idesc).map Hopcroft_DPDA_IDesc.fromCPSP = Hopcroft_DPDA.stepTransition (Hopcroft_DPDA.fromCPSP M) (Hopcroft_DPDA_IDesc.fromCPSP idesc) := by
+    let th : ∀ idesc, (CPSP_Transition.stepTransition M.transition idesc).map CPSP_DPDA_IDesc.toHopcroft = Hopcroft_DPDA.stepTransition (CPSP_DPDA.toHopcroft M) (CPSP_DPDA_IDesc.toHopcroft idesc) := by
       intro idesc
       exact CPSP_to_Hopcroft_preserves_semantics_single_step M idesc
     let rep := repeat_bind_map2 α β
-      Hopcroft_DPDA_IDesc.fromCPSP
-      (CPSP_Judge.stepTransition M.transition)
-      (Hopcroft_DPDA.stepTransition (Hopcroft_DPDA.fromCPSP M))
+      CPSP_DPDA_IDesc.toHopcroft
+      (CPSP_Transition.stepTransition M.transition)
+      (Hopcroft_DPDA.stepTransition (CPSP_DPDA.toHopcroft M))
       th
       n
       ⟨M.q0, w, []⟩
-    dsimp only [CPSP_DPDA.membership_provable_in_n_steps, CPSP_DPDA.run_n_steps, Hopcroft_DPDA.membership_provable_in_n_steps, Hopcroft_DPDA.run_n_steps, Hopcroft_DPDA_IDesc.fromCPSP]
-    dsimp only [Hopcroft_DPDA_IDesc.fromCPSP] at rep
-    rw [show (Hopcroft_DPDA.fromCPSP M).pda.q0 = M.q0 from rfl]
-    rw [show [(Hopcroft_DPDA.fromCPSP M).pda.z0] = List.map AugmentZ0.fromΓ [] ++ [AugmentZ0.z0] from rfl]
+    dsimp only [CPSP_DPDA.membership_provable_in_n_steps, CPSP_DPDA.run_n_steps, Hopcroft_DPDA.membership_provable_in_n_steps, Hopcroft_DPDA.run_n_steps, CPSP_DPDA_IDesc.toHopcroft]
+    dsimp only [CPSP_DPDA_IDesc.toHopcroft] at rep
+    rw [show (CPSP_DPDA.toHopcroft M).pda.q0 = M.q0 from rfl]
+    rw [show [(CPSP_DPDA.toHopcroft M).pda.z0] = List.map AugmentZ0.fromΓ [] ++ [AugmentZ0.z0] from rfl]
     simp only [Option.bind_eq_bind, List.map_nil, List.nil_append, Option.pure_def, Option.map_eq_map] at rep
     simp only [Option.bind_eq_bind, List.map_nil, List.nil_append]
     rw [rep]
-    simp only [Option.map, Hopcroft_DPDA.fromCPSP]
-    cases h : Nat.repeat (· >>= (CPSP_Judge.stepTransition M.transition)) n (some { p := M.q0, w := w, β := [] }) with
+    simp only [Option.map, CPSP_DPDA.toHopcroft]
+    cases h : Nat.repeat (· >>= (CPSP_Transition.stepTransition M.transition)) n (some { p := M.q0, w := w, β := [] }) with
     | none => rfl
     | some idesc => rfl
